SEARGroup.sml
@@ -1,7 +1,180 @@
-val Assoc_def = define_pred
-“!A m:A * A ~>A. Assoc(m) <=> 
- !a1 a2 a3. App(m,Pair(App(m,Pair(a1,a2)),a3)) = 
-App(m,Pair(a1,App(m,Pair(a2,a3))))”
+
+val mul_def = qdefine_fsym("mul",[‘m:G * G ->G’,‘g1:mem(G)’,‘g2:mem(G)’])
+‘App(m,Pair(g1,g2))’
+
+
+val asc_def = qdefine_psym("asc",[‘m:A * A -> A’])
+‘!a1 a2 a3. mul(m,mul(m,a1,a2),a3) = mul(m,a1,mul(m,a2,a3))’
+
+(*
+App(m,Pair(App(m,Pair(a1,a2)),a3)) = 
+App(m,Pair(a1,App(m,Pair(a2,a3))))’ |> gen_all
+*)
+
+val isunit_def = qdefine_psym("isunit",[‘m:A * A -> A’,‘e:mem(A)’])
+‘!a. mul(m,e,a) = a & mul(m,a,e) = a’
+
+
+val isinv_def = qdefine_psym("isinv",[‘m:A * A -> A’,‘i:A->A’,‘e:mem(A)’])
+‘!a. mul(m,App(i,a),a) = e & mul(m,a,App(i,a)) = e’
+
+
+
+(*c for component*)
+val c31_def = qdefine_fsym("c31",[‘abc:mem(A * B * C)’]) ‘Fst(abc)’
+val c32_def = qdefine_fsym("c32",[‘abc:mem(A * B * C)’]) ‘Fst(Snd(abc))’
+val c33_def = qdefine_fsym("c33",[‘abc:mem(A * B * C)’]) ‘Snd(Snd(abc))’
+
+val isgrp_def = qdefine_psym("isgrp",[‘g:mem(Exp(G * G,G) * Exp(G,G) * G)’])
+‘asc(tof(c31(g))) & 
+ isunit(tof(c31(g)),c33(g)) & 
+ isinv(tof(c31(g)),tof(c32(g)),c33(g))’
+
+val Grp_def = Thm_2_4 |> qspecl [‘Exp(G * G,G) * Exp(G,G) * G’]
+                      |> fVar_sInst_th “P(g:mem(Exp(G * G,G) * Exp(G,G) * G))”
+                         “isgrp(g:mem(Exp(G * G,G) * Exp(G,G) * G))”
+                      |> qSKOLEM "Grp" [‘G’]
+                      |> qSKOLEM "iG" [‘G’]
+
+val RepG_def = qdefine_fsym("RepG",[‘g:mem(Grp(G))’]) ‘App(iG(G),g)’
+
+val mof_def = qdefine_fsym("mof",[‘g:mem(Grp(G))’]) ‘tof(c31(RepG(g)))’
+val iof_def = qdefine_fsym("iof",[‘g:mem(Grp(G))’]) ‘tof(c32(RepG(g)))’
+val eof_def = qdefine_fsym("eof",[‘g:mem(Grp(G))’]) ‘c33(RepG(g))’
+
+val gmul_def = qdefine_fsym("gmul",[‘g:mem(Grp(G))’,‘x:mem(G)’,‘y:mem(G)’])
+‘mul(mof(g),x,y)’
+
+val ginv_def = qdefine_fsym("ginv",[‘g:mem(Grp(G))’,‘x:mem(G)’])
+‘App(iof(g),x)’
+
+val np_def = qdefine_fsym("np",[‘m:G * G ->G’,‘e:mem(G)’,‘x:mem(G)’])
+‘Nrec(e,Ap1(m,x))’
+
+val np_O = Nrec_O |> qsspecl [‘e:mem(G)’,‘Ap1(m:G * G->G,x)’]
+                  |> rewr_rule[GSYM np_def]
+
+val np_Suc = Nrec_Suc |> qsspecl [‘e:mem(G)’,‘Ap1(m:G * G->G,x)’,‘n:mem(N)’]
+                      |> rewr_rule[GSYM np_def]
+
+
+
+(*extend lambda tool into !z. ?n. .... ==> *)
+val Num_ex = proved_th $
+e0
+(cheat)
+(form_goal “!z. Lez(Oz,z) ==> ?!n. z = Asz(n,O)”)
+
+local 
+val th0 = proved_th $
+e0
+cheat
+(form_goal “?n:mem(N).T”)
+in 
+val Num_def = SKOLEM th0 "Num" [("z",mem_sort (rastt "Z"))] (Num_ex |> spec_all |> undisch |> uex2ex_rule) |> disch_all |> gen_all
+end
+
+val Ltz_def = qdefine_psym("Ltz",[‘z1:mem(Z)’,‘z2:mem(Z)’])
+‘Lez(z1,z2) & ~(z1 = z2)’ |> gen_all
+
+val zp_def = proved_th $
+e0
+cheat
+(form_goal 
+“!g:mem(Grp(G)). ?!f:G * Z -> G.
+ !gz. 
+ (Lez(Oz,Snd(gz)) ==> App(f,gz) = App(np(mof(g),eof(g),Fst(gz)),Num(Snd(gz)))) &
+ (Ltz(Snd(gz),Oz) ==> App(f,gz) = App(iof(g),App(np(mof(g),eof(g),Fst(gz)),Num(Negz(Snd(gz))))) )”)
+|> spec_all |> uex2ex_rule |> qSKOLEM "zp" [‘g’]
+
+val gpw_def = qdefine_fsym("gpw",[‘g:mem(Grp(G))’,‘x:mem(G)’,‘z:mem(Z)’])
+‘App(zp(g),Pair(x,z))’
+
+
+
+val cyc_def = qdefine_psym("cyc",[‘g:mem(Grp(G))’])
+‘?a. !x. ?z. x = gpw(g,a,z)’ |> gen_all
+
+(*can define a set Ghom(g1,g2), and say f:mem(Ghom(g1,g2)) ==> ...
+ but then run into the trouble with equalities.*)
+
+val ghom_def = qdefine_psym("ghom",[‘f:G1->G2’,‘g1:mem(Grp(G1))’,
+                                               ‘g2:mem(Grp(G2))’])
+‘!a b. App(f,gmul(g1,a,b)) = gmul(g2,App(f,a),App(f,b))’
+
+(*
+By the Division Theorem, it is possible to find integers 𝑞 and 𝑟 such that 𝑛=𝑚𝑞+𝑟 with 0≤𝑟<𝑚.
+*)
+
+val Subz_def = qdefine_fsym("Subz",[‘a:mem(Z)’,‘b:mem(Z)’])
+‘Addz(a,Negz(b))’
+
+val ghom_gpw = prove_store("ghom_gpw",
+e0
+(cheat)
+(form_goal “!f:G1 -> G2 g1 g2. ghom(f,g1, g2) ==>
+ !x z. App(f,gpw(g1,x,z)) = gpw(g2,App(f,x),z)”));
+
+val gpow_Mulz = prove_store("gpow_Mulz",
+e0
+cheat
+(form_goal
+ “!G g:mem(Grp(G)) a. gpw(g, a, Mulz(z1, z2)) = gpw(g, gpw(g, a, z1), z2)”));
+
+val Addz_eq_O = prove_store("Addz_eq_O",
+e0
+cheat
+(form_goal “!a b. Addz(a,b) = a <=> b = Oz”));
+
+val division_theorem = prove_store("division_theorem",
+e0
+cheat
+(form_goal 
+ “!a b:mem(Z).~(b = Oz) ==> ?!q r. a = Addz(Mulz(q,b),r) & 
+  Lez(Oz,r) & Lez(r,b)”));
+
+val sub_cyc_cyc = prove_store("sub_cyc_cyc",
+e0
+(rpt strip_tac >>
+ qcases ‘!x:mem(H). x = eof(h)’
+ >-- cheat >>
+ fs[cyc_def] >>
+ qby_tac ‘?m. ?x0. App(i,x0) = gpw(g,a,m) & Ltz(Oz,m) & 
+   !m'. ?x0. App(i,x0) = gpw(g,a,m') & Ltz(Oz,m') ==> Lez(m,m')  ’
+ >-- cheat >>
+ pop_assum strip_assume_tac >>
+ qexists_tac ‘x0’ >> strip_tac >>
+ qby_tac ‘?n. App(i,x) = gpw(g,a,n)’ 
+ >-- cheat >> pop_assum strip_assume_tac >>
+ qby_tac ‘~(m = )’
+ qby_tac
+ ‘?q r. n = Addz(Mulz(m,q),r)’ 
+ >-- cheat >>
+ pop_assum strip_assume_tac >> 
+ qsuff_tac ‘r = Oz’ 
+ >-- (strip_tac >> fs[Addz_Oz] >> qexists_tac ‘q’ >>
+     drule Inj_eq_eq >> first_x_assum (irule o iffLR) >> arw[] >>
+     drule ghom_gpw >> arw[] >> rw[gpow_Mulz]) >>
+ qsuff_tac ‘?x0. App(i,x0) = gpw(g,a,r)’ 
+ >-- strip_tac >>
+     first_x_assum (qspecl_then [‘r’] assume_tac) >> 
+     ccontra_tac >> 
+     
+
+
+ qsuff_tac ‘n = Mulz(m, q)’ 
+ >-- (* fs[] why loop?*) (once_arw[] >> rw[Addz_eq_O]) >>
+ 
+     )
+(form_goal “!H h:mem(Grp(H)) G g:mem(Grp(G)) i:H -> G.
+ ghom(i,h,g) & Inj(i) & cyc(g) ==> cyc(h)”)
+
+
+
+[‘h:mem(Pow(G))’,‘g:mem(Grp(G))’])
+‘is’
+
+
 
 
 val Grp0_def = define_pred
